ADTExamples/QueryStructure/ProcessScheduler/FMapExtensions.v
@@ -15,6 +15,27 @@ Module FMapExtensions_fun (E: DecidableType) (Import M: WSfun E).
   Definition GetValues {A: Type} (db: t A) : list A  :=
     List.map snd (elements db).
 
+  Definition FindWithDefault {A: Type} (key: key) (db: t A) (default: A) :=
+    match find key db with
+      | Some x => x
+      | None   => default
+    end.
+  
+  Definition IndexedBy {A} projection tree :=
+    forall key (value: A),
+      MapsTo key value tree ->
+      key = projection value.
+
+  Lemma FindWithDefault_MapsTo :
+    forall {A} default key (value: A) tree,
+      MapsTo key value tree -> 
+      FindWithDefault key tree default = value.
+  Proof.
+    unfold FindWithDefault; intros ? ? ? ? ? maps_to.
+    rewrite find_mapsto_iff in *.
+    rewrite maps_to; trivial.
+  Qed.
+
   Definition ValueFilter {A B: Type} (pred: B -> bool) :=
     (fun (key: A) (value: B) => pred value).
 
@@ -262,6 +283,20 @@ Module FMapExtensions_fun (E: DecidableType) (Import M: WSfun E).
     eauto using in_elements_after_add, in_elements_after_add'.
   Qed.
 
+
+  Lemma In_MapsTo : 
+    forall A tree key,
+      In key tree -> 
+      exists (value: A), 
+        (MapsTo key value tree /\ find key tree = Some value).
+  Proof.
+    intros A tree key H;
+    apply in_find_iff in H;
+    destruct (find key tree) as [value | ] eqn:eq_option;
+    try rewrite <- find_mapsto_iff in eq_option;
+    intuition eauto.
+  Qed.
+
   Lemma EnsembleListEquivalence_fmap_add_filtered :
     forall {A: Type} (cond : A -> Prop) ensemble key tree added,
       cond added ->
@@ -290,3 +325,121 @@ Module FMapExtensions_fun (E: DecidableType) (Import M: WSfun E).
 End FMapExtensions_fun.
 
 Module FMapExtensions (M: WS) := FMapExtensions_fun M.E M.
+
+Module NestedTrees (M1: WS) (M2: WS).
+  Module Ext1 := FMapExtensions M1.
+  Module Ext2 := FMapExtensions M2.
+
+  Definition PartitionedEnsembleListEquivalence {A} set_db tree_db projection :=
+      forall key_instance,
+        EnsembleListEquivalence
+          (FilteredSet set_db projection key_instance)
+          (@Ext2.GetValues A (Ext1.FindWithDefault key_instance tree_db (M2.empty A))).
+
+
+  Definition ExtractRows {A: Type} db :=
+    @flatten A (map Ext2.GetValues 
+                    (Ext1.GetValues db)).
+
+  Lemma FindWithDefault_NonEmpty_Found :
+    forall {A} key tree,
+      let subtree := Ext1.FindWithDefault key tree (M2.empty A) in
+      (exists row, List.In row (Ext2.GetValues subtree)) ->
+      List.In subtree (Ext1.GetValues tree).
+  Proof.    
+    intros.
+    unfold Ext1.FindWithDefault in subtree.
+    destruct (M1.find key tree) eqn:eq_find.
+
+    rewrite <- Ext1.BasicFacts.find_mapsto_iff in eq_find.
+    unfold Ext1.GetValues.
+    rewrite <- Ext1.MapsTo_snd.
+    eauto.
+
+    exfalso.
+    destruct H as [row row_in].
+    unfold Ext2.GetValues in row_in.
+    rewrite <- Ext2.MapsTo_snd in row_in. (* TODO: Embed GetValues in MapsTo_snd *)
+    destruct row_in as [key2 maps_to].
+    rewrite <- Ext2.BasicFacts.empty_mapsto_iff.
+    eauto.
+  Qed.
+
+  Definition IndexedBy {A} projection tree :=
+    forall key subtree,
+      M1.MapsTo key subtree tree ->
+      forall (row: A),
+        List.In row (Ext2.GetValues subtree) -> projection row = key. 
+
+  Lemma unpartition :
+    forall {A} projection set_db tree_db,
+      IndexedBy projection tree_db ->
+      @PartitionedEnsembleListEquivalence A set_db tree_db projection ->
+      EnsembleListEquivalence set_db (ExtractRows tree_db).
+    Proof.
+      unfold PartitionedEnsembleListEquivalence, ExtractRows; intros.
+      unfold EnsembleListEquivalence; intros.
+
+      specialize (H0 (projection x)).
+      unfold FilteredSet in *.
+      unfold ExtractRows.
+
+      split; intros.
+      rewrite in_flatten_iff.
+      set (subtree := (Ext1.FindWithDefault (projection x) tree_db (M2.empty A))) in *.
+      exists (Ext2.GetValues subtree).
+      
+      specialize (H0 x); unfold Ensembles.In in *; simpl in H0.
+      rewrite in_map_iff.
+      split.
+      
+      intuition.
+      exists subtree; split; trivial.
+      destruct H0 as (H0 & _).
+
+      Lemma ugh: 
+        forall (P Q R: Prop),
+         (P /\ Q -> R) <->  (P -> Q -> R).
+      Proof.
+        tauto.
+      Qed.
+      
+      rewrite ugh in H0.
+      specialize (H0 H1 (eq_refl (projection x))).
+ 
+      apply FindWithDefault_NonEmpty_Found;
+        eauto.
+
+      specialize (H0 x).
+      destruct H0 as (_ & H0).
+
+      unfold Ensembles.In in *.
+
+      Lemma ugh2 :
+        forall (P Q R: Prop),
+          (P -> (Q /\ R)) <-> ((P -> Q) /\ (P -> R)).
+      Proof.
+        tauto.
+      Qed.
+
+      rewrite ugh2 in H0.
+      destruct H0 as (H0 & _).
+
+      rewrite in_flatten_iff in H1.
+      destruct H1 as [subtree_values (x_in_subtree_values & subtree_values_in_map)].
+      rewrite in_map_iff in subtree_values_in_map.
+      destruct subtree_values_in_map as [subtree (subtree_values_correct & subtree_in_tree_values)].
+      unfold Ext1.GetValues in subtree_in_tree_values.
+      rewrite <- Ext1.MapsTo_snd in subtree_in_tree_values.
+      destruct subtree_in_tree_values as [key maps_to].
+      subst.
+
+      unfold IndexedBy in H.
+      specialize (H _ _ maps_to _ x_in_subtree_values).
+      subst.
+
+      apply (Ext1.FindWithDefault_MapsTo (M2.empty A)) in maps_to.
+      rewrite maps_to in H0.
+      intuition.
+    Qed.
+End NestedTrees.
